fairneris/fuel_jm_scheduling_fairness.v
@@ -1,0 +1,32 @@
+From fairneris Require Import fairness fuel env_model env_model_project.
+
+
+Section upto.
+  Context {Λ: language}.
+  Context `{GoodLang Λ}.
+  Context {M: UserModel Λ}.
+  Context {N: EnvModel Λ}.
+  Context {LM: LiveModel Λ (joint_model M N)}.
+
+
+  (* TODO: remove this, this is just a translation between two definitions of fairness. *)
+
+  Lemma upto_stutter_fairness_ltl (auxtr: auxtrace LM) (mtr: mtrace (joint_model M N)):
+    upto_stutter_aux auxtr mtr ->
+    (∀ ρ, fair_aux (LM := LM) ρ auxtr) →
+    jm_fair_scheduling mtr.
+  Proof.
+    intros Hupto Hfair ρ.
+    opose proof (upto_stutter_fairness auxtr mtr _ _ (ρ: fmrole (joint_model M N))) as Hf=>//.
+    rewrite /fairness.fair_scheduling_mtr /jm_fair_scheduling_mtr in Hf *.
+    rewrite /trace_always_eventually_implies_now /trace_always_eventually_implies.
+    rewrite trace_alwaysI. intros tr' [n Hsuff]. rewrite trace_impliesI. intros Hnow.
+    rewrite /trace_utils.trace_implies in Hf. odestruct (Hf n _) as [m Hm].
+    { rewrite /pred_at Hsuff. done. }
+    rewrite /pred_at in Hm.
+    rewrite trace_eventuallyI.
+    destruct (after (n+m) mtr) as [mtr'|] eqn:Heq; rewrite Heq in Hm; last naive_solver.
+    exists mtr'; split; last naive_solver.
+    exists m. rewrite after_sum' Hsuff // in Heq.
+  Qed.
+End upto.
